Complete interop wrapper for aes128 key expansion

vale/code/crypto/aes/x64/Main.ml
@@ -2,10 +2,10 @@ let _ =
   CmdLineParser.parse_cmdline [
       ("aes128_key_expansion", (fun win -> X64_AES.va_code_KeyExpansionStdcall win AES_s.AES_128));
       ("aes256_key_expansion", (fun win -> X64_AES.va_code_KeyExpansionStdcall win AES_s.AES_256));
-      ("gcm128_encrypt0",       (fun win -> X64_GCMencrypt.va_code_gcm_encrypt_stdcall win AES_s.AES_128));
+(*      ("gcm128_encrypt0",       (fun win -> X64_GCMencrypt.va_code_gcm_encrypt_stdcall win AES_s.AES_128)); *)
       ("gcm128_encrypt",       (fun win -> X64_GCMencrypt.va_code_gcm_encrypt2_stdcall win AES_s.AES_128));
       ("gcm128_decrypt",       (fun win -> X64_GCMdecrypt.va_code_gcm_decrypt_stdcall win AES_s.AES_128));
-      ("gcm256_encrypt0",       (fun win -> X64_GCMencrypt.va_code_gcm_encrypt_stdcall win AES_s.AES_256));
+(*      ("gcm256_encrypt0",       (fun win -> X64_GCMencrypt.va_code_gcm_encrypt_stdcall win AES_s.AES_256)); *)
       ("gcm256_encrypt",       (fun win -> X64_GCMencrypt.va_code_gcm_encrypt2_stdcall win AES_s.AES_256));
       ("gcm256_decrypt",       (fun win -> X64_GCMdecrypt.va_code_gcm_decrypt_stdcall win AES_s.AES_256));
       ("gcm128_encrypt_opt",       (fun win -> X64_GCMencryptOpt.va_code_gcm_blocks_stdcall win AES_s.AES_128));
