vale/code/arch/x64/interop/Gcm_simplify.fsti
@@ -42,3 +42,12 @@ val gcm_simplify3 (b:buf_t TUInt8 TUInt128) (h:HS.mem) : Lemma
       (seq_uint8_to_seq_nat8 (B.as_seq h b))
       (be_quad32_to_bytes (reverse_bytes_quad32 (low_buffer_read TUInt8 TUInt128 h b 0)))
   ))
+
+val aes_simplify1 (b:buf_t TUInt8 TUInt128) (h:HS.mem) : Lemma 
+  (requires B.live h b /\ B.length b = 16)
+  (ensures (
+  DV.length_eq (get_downview b);
+  Seq.equal
+    (seq_nat8_to_seq_nat32_LE (seq_uint8_to_seq_nat8 (B.as_seq h b)))
+    (quad32_to_seq (low_buffer_read TUInt8 TUInt128 h b 0))
+  ))
