Makefile
@@ -633,7 +633,7 @@ DEFAULT_FLAGS		=\
   -bundle EverCrypt.BCrypt \
   -bundle EverCrypt.OpenSSL \
   -bundle MerkleTree.Spec,MerkleTree.Spec.*,MerkleTree.New.High,MerkleTree.New.High.* \
-  -bundle 'Vale.Stdcalls.*,Interop,Interop.*,Fadd_stdcalls,Cpuid_stdcalls,Fswap_stdcalls,Fmul_stdcalls,Fsqr_stdcalls,Fsub_stdcalls,Poly_stdcalls,Sha_stdcalls[rename=Vale]' \
+  -bundle 'Vale.Stdcalls.*,Interop,Interop.*,Fadd_stdcalls,Cpuid_stdcalls,Fswap_stdcalls,Fmul_stdcalls,Fsqr_stdcalls,Fsub_stdcalls,Poly_stdcalls,Sha_stdcalls,GCMencrypt_stdcalls,GCMencryptOpt_stdcalls,AES_stdcalls[rename=Vale]' \
   -bundle 'Fadd_inline,Fmul_inline,Fsqr_inline,Fswap_inline[rename=Vale_Inline]' \
   -bundle FStar.Tactics.CanonCommMonoid,FStar.Tactics.CanonCommSemiring,FStar.Tactics.CanonCommSwaps[rename=Unused] \
   -bundle FastUtil_helpers,FastHybrid_helpers,FastSqr_helpers,FastMul_helpers[rename=Unused2] \
